# 数学公式

## 微积分

$ \lim \limits_{x \to x_0} f(x) = A $

$ \lim \limits_{x \to x_0} f(x) = A \Leftrightarrow \lim \limits_{x \to x_0^-} f(x) = \lim \limits_{x \to x_0^+} f(x) = A$

$$ \alpha θ \theta o o τ \tau β \beta ϑ \vartheta π \pi υ \upsilon γ \gamma ι \iota \varpi φ \phi δ \delta κ \kappa ρ \rho ϕ \varphi  \epsilon λ \lambda % \varrho χ \chi ε \varepsilon µ \mu σ \sigma ψ \psi ζ \zeta ν \nu ς \varsigma ω \omega η \eta ξ \xi
Γ \Gamma Λ \Lambda Σ \Sigma Ψ \Psi $$
$$
\lim \limits_{x \to 0^-}f(x) \ne \lim \limits_{x \to x_0^+} f(x) \rightarrow \lim \limits_{x \to x^0} f(x)  不存在\\
\lim \limits_{x \to 0^-} \frac{|x|}{x}= -1 \ne \lim \limits_{x \to 0^+} \frac{|x|}{x} = 1 \rightarrow \lim \limits_{x \to 0} \frac{|x|}{x} 不存在\\
\lim \limits_{x \to -\infty} a^x = \infty , and \lim \limits_{x \to \infty } a^x = 0 \space\space when \space a > 1 \\
\lim \limits_{x\to 0}(1+x)^{\frac{1}{x}} = \lim \limits_{x \to \infty}(1+\frac{1}{x})^x = e\\
\lim \limits_{x \to x_0}\frac{f(x)}{g(x)}=\frac{A}{B} \space\space\space  (B \ne 0)\\
\lim \limits_{x \to \sim}\frac{f(x)}{g(x)} = \lim \limits_{x \to \sim}\frac{f'(x)}{g'(x)}\\
\lim \limits_{x \to \pm\infty}=\pm\infty\\
f'(x_0) = \lim \limits_{h \to 0}\frac{f(x_0+h)-f(x_0)}{h}= \lim \limits_{x \to x_0}\frac{f(x)-f(x_0)}{x-x_0}\\
f'(x_0)=A \leftrightarrow f'_-(x_0) = f'_+(x_0) = A \\
y'(x_0)=f'(x_0)=\frac{dy}{dx}\mid_{x=x_0}\\
(sinx)'=cosx \space (secx)'=secx\cdot tanx\\
\frac{d^2y}{dx^2}=\frac{\frac{d(\frac{dy}{dx})}{dt}}{\frac{dx}{dt}}\\
distance = \int_{a}^{b}|v(t)|dt\\
displacement = \int_{a}^{b}v(t)dt\\
speed = \sqrt{(x'(t))^2+(y'(t))^2}\\
\int\frac{(x^{1/3}-4)^5}{6x^{2/3}}dx\\
\int_{-\infty}^{\infty}f(x)dx = \lim \limits_{a \to -\infty}\int_{a}^{c}f(x)dx+\lim \limits_{b \to +\infty}\int_{c}^{b}f(x)dx\\

\frac{dy}{dx}+P(x)y=Q(x)\\
\left. \frac{{\rm d}y}{{\rm d}x} \right|_{x=0}=3x+1=1\\
y''+py'+qy=f(x)\\
\frac{\partial u}{\partial t}= h^2 \left( \frac{\partial^2 u}{\partial x^2} +\frac{\partial^2 u}{\partial y^2}+ \frac{\partial^2 u}{\partial z^2}\right)\\
A=\begin{bmatrix}
{a_{11}}&{a_{12}}&{\cdots}&{a_{1n}}\\
{a_{21}}&{a_{22}}&{\cdots}&{a_{2n}}\\
{\vdots}&{\vdots}&{\ddots}&{\vdots}\\
{a_{m1}}&{a_{m2}}&{\cdots}&{a_{mn}}\\
\end{bmatrix}\\
D=\begin{vmatrix}
{a_{11}}&{a_{12}}&{\cdots}&{a_{1n}}\\
{a_{21}}&{a_{22}}&{\cdots}&{a_{2n}}\\
{\vdots}&{\vdots}&{\ddots}&{\vdots}\\
{a_{m1}}&{a_{m2}}&{\cdots}&{a_{mn}}\\
\end{vmatrix}\\
\begin{array}{c|lll}
{}&{a}&{b}&{c}\\
\hline
{R_1}&{c}&{b}&{a}\\
{R_2}&{b}&{c}&{c}\\
\end{array}\\
\sin60^\omicron \\
f(x) \,\!
= \sum_{n=0}^\infty a_n x^n = a_0+a_1x+a_2x^2+\cdots
$$




$ \begin{align} a=(1+2+3+4+5+6+7+8+9+10)   \end{align} $

 

$ \frac{\mathrm{d} y }{\mathrm{d} x} $   $ \frac{\mathrm{d}^{n} y }{\mathrm{d} x^{n}} $  

$ \frac{\partial f}{\partial x} $  $ \frac{\partial ^{n} f}{\partial x^{n}} $  $ \frac{ \dot y }{ \dot x } $ $ \frac{ \ddot y }{ \ddot x } $  $  \frac{ \dddot y }{ \dddot x } $    $  \frac{du}{dt}  and  \frac{d^2 u}{dx^2}  $

$ \lim \limits_{x \to \infty} \frac{a^x+(1+c^3)}{b^x}$

$ x_i y_i$  $ \frac{ y^{'} }{ x^{'} } $

$$ h(\theta) = \sum_{j=0} ^n \theta_j x_j $$

$$ \begin{equation} 
X(k)=\sum_{n=0}^{N-1} x(n)e^{-j \frac{2 \pi}{N} k n}=\sum_{n=0}^{N-1} x(n) W_N^{kn},\quad k=0,1,...,N-1. 
\end{equation} $$ 

$$ \begin{align} \frac{\partial J(\theta)}{\partial\theta_j} & = -\frac1m\sum_{i=0}^m(y^i - h_\theta(x^i)) \frac{\partial}{\partial\theta_j}(y^i-h_\theta(x^i))\\ & = -\frac1m\sum_{i=0}^m(y^i-h_\theta(x^i)) \frac{\partial}{\partial\theta_j}(\sum_{j=0}^n\theta_j x^i_j-y^i)\\ &=-\frac1m\sum_{i=0}^m(y^i -h_\theta(x^i)) x^i_j \end{align} $$

$$ \frac{\partial J(\theta)}{\partial\theta_j} = -\frac1m\sum_{i=0}^m(y^i - 	h_\theta(x^i))x^i_j $$

$$ J(\theta) = \frac{1}{2m}\sum_{i=0}^m(y^i - h_\theta(x^i))^2 $$

\$$ H_c=\sum_{l_1+\dots +l_p}\prod^p_{i=1} \binom{n_i}{l_i} \$$

$$ f(n)= \begin{cases} 	n/2, & \text{if $n$ is even}\\ 	3n+1,& \text{if $n$ is odd} \end{cases} $$

$$ \begin{matrix} 1 & x & x^2\\ 1 & y & y^2\\ 1 & z & z^2\\ \end{matrix} $$

 $ \displaystyle \int_{1}^{\frac{pi}{2}} 2xdx= 0 $ 

$ \displaystyle \int_{1}^{10} f^{-1}(x)dx $

##  希腊字母

$$
A	A	α \alpha α	\alpha \\
B B B	B	β \beta β	\beta \\
Γ \Gamma Γ	\Gamma	γ \gamma γ	\gamma \\
Δ \Delta Δ	\Delta	δ	\delta \\
E E E	E	ϵ \epsilon ϵ	\epsilon \\
Z Z Z	Z	ζ \zeta ζ	\zeta \\
H H H	H	η \eta η	\eta \\
Θ \Theta Θ	\Theta	θ \theta θ	\theta \\
I I I	I	ι \iota ι	\iota \\
K K K	K	κ \kappa κ	\kappa\\
Λ \Lambda Λ	\Lambda	λ \lambda λ	\lambda\\
M M M	M	μ \mu μ	\mu\\
N N N	N	ν \nu ν	\nu\\
Ξ \Xi Ξ	\Xi	ξ \xi ξ	\xi\\
O O O	O	ο \omicron ο	\omicron\\
Π \Pi Π	\Pi	π \pi π	\pi\\
P P P	P	ρ \rho ρ	\rho\\
Σ \Sigma Σ	\Sigma	σ \sigma σ	\sigma\\
T T T	T	τ \tau τ	\tau\\
Υ \Upsilon Υ	\Upsilon	υ \upsilon υ	\upsilon\\
Φ \Phi Φ	\Phi	ϕ \phi ϕ	\phi\\
X X X	X	χ \chi χ	\chi\\
Ψ \Psi Ψ	\Psi	ψ \psi ψ	\psi\\
Ω \Omega Ω	\Omega	ω \omega ω	\omega\\
$$





# 化学方程式

$A\underset{0^{\circ}C }{\overset{100^{\circ}C}{\rightleftarrows}}B$

$ 2H_2 + O_2 \xrightarrow{n,m}2H_2O $

$ \ce{2H2 + O2 ->[\Delta] H2O} $

$ \ce{N2 + 3H2 <=>T[高温、加压][催化剂] 2NH3}$

$ \ce{KCr(SO4)2 * 12H2O}$ 

$\ce{SO4^2- + Ba^2+ -> BaSO4 v}$

$ \ce{Ca(OH)2 + CO2 = CaCO3 v + H2O}$

$ \underset{\text{葡萄糖}}{\ce{C6H12O6}} $

$  \ce{Fe + 2H+ = H2 ^ + Fe^2+} $

# 其他公式

$ \Gamma(z) = \int_0^\infty t^{z-1}e^{-t}dt\,.$

$y_k=\varphi(u_k+v_k)$ 

$y(x)=x^3+2x^2+x+1$ 

$x^{y}=(1+{\rm e}^x)^{-2xy}$ 

$\displaystyle f(n)=\sum_{i=1}^{n}{n*(n+1)}$

$$y=\begin{cases} 2x+1, & x \leq0\\ x, & x>0 \end{cases}$$

$$ \left \{  \begin{array}{c} a_1x+b_1y+c_1z=d_1 \\  a_2x+b_2y+c_2z=d_2 \\  a_3x+b_3y+c_3z=d_3 \end{array} \right. $$

$$ \int_{\theta_1(x)}^{\theta_2(x)}=l $$

$$\iint dx dy=\sigma$$

$$\iiint dx dydz=\nu$$

$$\frac{dy}{dx}+P(x)y=Q(x)$$ 

$\left. \frac{{\rm d}y}{{\rm d}x} \right|_{x=0}=3x+1=1 $

$$y''+py'+qy=f(x)$$ 

$$\frac{d^2y}{dx^2}+p\frac{dy}{dx}+qy=f(x)$$

$$ \frac{\partial u}{\partial t}= h^2 \left( \frac{\partial^2 u}{\partial x^2} +\frac{\partial^2 u}{\partial y^2}+ \frac{\partial^2 u}{\partial z^2}\right) $$

$$\begin{bmatrix} 1&0&0\\ 0&1&0\\ 0&0&1\\ \end{bmatrix} $$

$$ \left[  \begin{array}  {c c | c}  1 & 2 & 3 \\ \hline  4 & 5 & 6 \end{array}  \right] $$

$$ f(n)=\lim \limits_{n \rightarrow +\infty} \frac{1}{n(n+1)}$$

 $$\frac{1}{\lim_{u \rightarrow \infty}}, \frac{1}{\lim\limits_{u \rightarrow \infty}} $$

$ \lbrace x-y \rbrace $

$ \sin(x)   \cos(x)   \tan(x)  \log_2 10  \ln2 $

## 向量

$ \vec{a} \bar{a}\hat{a}\overline{xyz}$

$ \displaystyle \sum^{x \to \infty}_{y \to 0}{\frac{x}{y}} $

$ \overbrace{a+b+c} $

## 其他

$$
\left\{
\begin{aligned}
x_1+2x_2&=3\\
2x_1-x_2&=1\\
\end{aligned}
\right.
\\
\begin{aligned}
y&=x^2+4x+4\\
&=(x+2)^2\\
\end{aligned}
\\
\sin\theta  \\
arcsin\frac{L}{r} \\
\operatorname{argsh}k\\
\operatorname{argth}m\\
\sqrt[n]{3}\\
因为\because 所以\therefore\\
\angle\Alpha\Beta\Gamma\P\imath\ell\mho\\
{}_1^2\!X_3^4 \\
x^\prime \\
\\
\overleftarrow{a b}\overrightarrow{c d}\\
\\
\begin{matrix} 5050 \\ \overbrace{ 1+2+\cdots+100 }\end{matrix}\\
\begin{matrix} \underbrace{ a+b+\cdots+z } \\ 26\end{matrix}\\
\begin{matrix} \coprod_{i=1}^N x_i\end{matrix}\\
\oint_{C} x^3\, dx + 4y^2\, dy\\
\dbinom{n}{r}=\binom{n}{n-r}=C^n_r=C^n_{n-r}\\
\tbinom{n}{r}=\tbinom{n}{n-r}=C^n_r=C^n_{n-r}	\\
\begin{Vmatrix}
x & y \\
z & v
\end{Vmatrix}\\
\begin{Bmatrix}
x & y \\
z & v
\end{Bmatrix}\\
f(n) =
\begin{cases} 
n/2,  & \mbox{if }n\mbox{ is even} \\
3n+1, & \mbox{if }n\mbox{ is odd}
\end{cases}\\
\begin{align}
f(x) & = (m+n)^2 \\
& = m^2+2mn+n^2 \\
\end{align}\\
\mathbb{ABCDEFGHIJKLMNOPQRSTUVWXYZ}\\
\mathbf{012…abc…ABC…}\\
\left( \frac{1}{2} \right)\\
\left( \frac{a}{b} \right)\left[ \frac{a}{b} \right]\left\{ \frac{a}{b} \right\}\\
\Bigg ( \bigg [ \Big \{\big\langle \left | \| \frac{a}{b} \| \right | \big \rangle\Big\}\bigg ] \Bigg )\\

{\color{Blue}x^2}+{\color{Brown}2x} -{\color{OliveGreen}1}\\
x_{\color{Maroon}1,2}=\frac{-b\pm\sqrt{{\color{Maroon}b^2-4ac}}}{2a}\\
2x=1 \,通过png图显示出来\\

\begin{aligned}
 \sigma_1 &= x + y  &\quad \sigma_2 &= \frac{x}{y} \\
 \sigma_1' &= \frac{\partial x + y}{\partial x} 
 & \sigma_2' 
    &= \frac{\partial \frac{x}{y}}{\partial x}
\end{aligned}\\

\begin{aligned}
a_0&=\frac{1}{\pi}\int\limits_{-\pi}^{\pi}f(x)\,\mathrm{d}x\\[6pt]
a_n&=\frac{1}{\pi}\int\limits_{-\pi}^{\pi}f(x)\cos nx\,\mathrm{d}x=\\
&=\frac{1}{\pi}\int\limits_{-\pi}^{\pi}x^2\cos nx\,\mathrm{d}x\\[6pt]
b_n&=\frac{1}{\pi}\int\limits_{-\pi}^{\pi}f(x)\sin nx\,\mathrm{d}x=\\
&=\frac{1}{\pi}\int\limits_{-\pi}^{\pi}x^2\sin nx\,\mathrm{d}x
\\[6pt]
\end{aligned}\\

z = \overbrace{
   \underbrace{x}_\text{real} + i
   \underbrace{y}_\text{imaginary}
  }^\text{complex number}\\
  
f(x) = \left\{
  \begin{array}{lr}
    x^2 & : x < 0\\
    x^3 & : x \ge 0
  \end{array}
\right.
\\
u(x) = 
  \begin{cases} 
   \exp{x} & \text{if } x \geq 0 \\
   1       & \text{if } x < 0
  \end{cases}\\
 
 h(\theta) = \sum_{j = 0} ^n \theta_j x_j  \\
 
\begin{aligned}
 \boxed{x^2+y^2 = z^2}
\end{aligned}\\

\begin{gathered}
\operatorname{arg\,max}_a f(a) 
 = \operatorname{*}{arg\,max}_b f(b) \\
 \operatorname{arg\,min}_c f(c) 
 = \operatorname {*}{arg\,min}_d f(d)
\end{gathered}\\

\begin{aligned}
   \sum\nolimits' C_n
\end{aligned}\\
\begin{aligned}
   \sum_{n=1}\nolimits' C_n
\end{aligned}\\
\begin{aligned}
   \sideset{}{'}\sum_{n=1}C_n
\end{aligned}\\

\begin{aligned}
   \sideset{_a^b}{_c^d}\sum
\end{aligned}\\

\prod_{{
  \begin{gathered}
            1\le i \le n\\
            1\le j \le m
  \end{gathered}
            }}
     M_{i,j}\\
$$
---

代码块
``` Java
import java.*;

public class MyClass{
    public static void main(String[] args){
        System.out.println("Hello world!");
    }
}
```

$$
\pm                  \cap                \diamond                    \oplus      
 \mp                  \cup                \bigtriangleup              \ominus     
 \times               \uplus              \bigtriangledown            \otimes     
 \div                 \sqcap              \triangleleft               \oslash     
 \ast                 \sqcup              \triangleright              \odot       
 \star                \vee                \lhd$^b$                    \bigcirc    
 \circ                \wedge              \rhd$^b$                    \dagger     
 \bullet              \setminus           \unlhd$^b$                  \ddagger    
 \cdot                \wr                 \unrhd$^b$                  \amalg \\
 \\
 \leq                 \geq                \equiv              \models       
 \prec                \succ               \sim                \perp         
 \preceq              \succeq             \simeq              \mid          
 \ll                  \gg                 \asymp              \parallel     
 \subset              \supset             \approx             \bowtie       
 \subseteq            \supseteq           \cong               \Join$^b$     
 \sqsubset$^b$        \sqsupset$^b$       \neq                \smile        
 \sqsubseteq          \sqsupseteq         \doteq              \frown        
 \in                  \ni                 \propto \\
 \\
 \colon              \ldotp              \cdotp  \\
 \leftarrow                   \longleftarrow              \uparrow      
 \Leftarrow                   \Longleftarrow              \Uparrow      
 \rightarrow                  \longrightarrow             \downarrow    
 \Rightarrow                  \Longrightarrow             \Downarrow    
 \leftrightarrow              \longleftrightarrow         \updownarrow  
 \Leftrightarrow              \Longleftrightarrow         \Updownarrow  
 \mapsto                      \longmapsto                 \nearrow      
 \hookleftarrow               \hookrightarrow             \searrow      
 \leftharpoonup               \rightharpoonup             \swarrow      
 \leftharpoondown             \rightharpoondown           \nwarrow      
 \rightleftharpoons           \leadsto  \\
 \ldots               \cdots              \vdots              \ddots        
 \aleph               \prime              \forall             \infty        
 \hbar                \emptyset           \exists             \Box$^b$      
 \imath               \nabla              \neg                \Diamond$^b$  
 \jmath               \surd               \flat               \triangle     
 \ell                 \top                \natural            \clubsuit     
 \wp                  \bot                \sharp              \diamondsuit  
 \Re                  \|                  \backslash          \heartsuit    
 \Im                  \angle              \partial            \spadesuit    
 \mho \\
 \sum                 \bigcap             \bigodot      
 \prod                \bigcup             \bigotimes    
 \coprod              \bigsqcup           \bigoplus     
 \int                 \bigvee             \biguplus     
 \oint                \bigwedge \\
 \arccos     \cos       \csc      \exp      \ker         \limsup      \min      \sinh  \\
 \arcsin     \cosh      \deg      \gcd      \lg          \ln	      \Pr       \sup   \\
 \arctan     \cot       \det      \hom      \lim         \log	      \sec      \tan   \\
 \arg        \coth      \dim      \inf      \liminf      \max	      \sin      \tanh \\
 
  (                    )                   \uparrow            \Uparrow      
 [                    ]                   \downarrow          \Downarrow    
 \{                   \}                  \updownarrow        \Updownarrow  
 \lfloor              \rfloor             \lceil              \rceil        
 \langle              \rangle             /                   \backslash    
 |                    \|
 \\
 \rmoustache        \lmoustache         \rgroup            \lgroup 
  \arrowvert         \Arrowvert          \bracevert
 \\
 \hat{a}            \acute{a}         \bar{a}           \dot{a}           \breve{a} 
 \check{a}          \grave{a}         \vec{a}           \ddot{a}          \tilde{a} \\
 \widetilde{abc}                     \widehat{abc}
 \overleftarrow{abc}                 \overrightarrow{abc}
 \overline{abc}                      \underline{abc}
 \overbrace{abc}                     \underbrace{abc}
 \sqrt{abc}                          \sqrt[n]{abc}
 $f'$                                \frac{abc}{xyz} \\
 \\
 \mathcal{ABCDEFG}\\
 \mathfrak{ABCDEFGabcdefghigh}\\
 \alpha               \theta               o                  \tau          
 \beta                \vartheta           \pi                 \upsilon      
 \gamma               \gamma              \varpi              \phi          
 \delta               \kappa              \rho                \varphi       
 \epsilon             \lambda             \varrho             \chi          
 \varepsilon          \mu                 \sigma              \psi          
 \zeta                \nu                 \varsigma           \omega        
 \eta                 \xi                                           
                                                                 
 \Gamma               \Lambda             \Sigma              \Psi          
 \Delta               \Xi                 \Upsilon            \Omega        
 \Theta               \Pi                 \Phi
 \\
 \begin{aligned}
  \item $J(\theta)=\sum_{i=0}^{m} (h_{\theta}(x_i)-y_i)^2$
  \item $$J(\theta)=\sum_{i=0}^{m} (h_{\theta}(x_i)-y_i)^2$$
  \item $J(\theta)=\sum\limits_{i=0}^{m} (h_{\theta}(x_i)-y_i)^2$
  \item $ \sum\limits_{i=1} $
  \item $ \mathop{\theta}\limits_{i=1}^2 $
\end{aligned}
$$

方法一： $$ f(x)=\left\{ \begin{aligned} x & = & \cos(t) \\ y & = & \sin(t) \\ z & = & \frac xy \end{aligned} \right. $$ 

方法二： $$ F^{HLLC}=\left\{ \begin{array}{rcl} F_L       &      & {0      <      S_L}\\ F^*_L     &      & {S_L \leq 0 < S_M}\\ F^*_R     &      & {S_M \leq 0 < S_R}\\ F_R       &      & {S_R \leq 0} \end{array} \right. $$

 方法三: $$f(x)= \begin{cases} 0& \text{x=0}\\ 1& \text{x!=0} \end{cases}$$

